reflection of sexprs, almost consumable.

src/ndep/SepExpr.v
@@ -370,4 +370,562 @@ Module SepExpr (B : Heap) (ST : SepTheoryX.SepTheoryXType B).
 
   End env.
 
+  Implicit Arguments Func [ types pcType stateType ].
+  Implicit Arguments Exists [ types pcType stateType ].
+  Implicit Arguments Star [ types pcType stateType ].
+
+  (** Reflection **)
+  Require Import Reflect.
+
+  Ltac extend_type T D types :=
+    match T with
+      | Prop => types
+      | _ => 
+        let rec find types :=
+        match types with
+          | nil => constr:(false)
+          | ?a :: ?b =>
+            let T' := eval simpl Impl in (Impl a) in
+            match T' with
+              | T => constr:(true)
+              | _ => find b
+            end
+        end
+        in
+        match find types with
+          | true => types
+          | _ => constr:(D :: types)
+        end
+    end.
+
+  Definition defaultType (T : Type) : type :=
+    {| Impl := T; Eq := fun _ _ => None |}.
+
+  Ltac extend_all_types Ts types :=
+    match Ts with
+      | nil => types
+      | ?a :: ?b => 
+        let types := extend_type a (defaultType a) types in
+        extend_all_types b types
+    end.  
+
+  Record VarType (t : Type) : Type :=
+    { open : t }.
+  Definition openUp T U (f : T -> U) (vt : VarType T) : U :=
+    f (open vt).
+
+  Ltac collectTypes_expr e types :=
+    match e with
+      | fun x => (@openUp _ ?T _ x) =>
+        let v := constr:(T:Type) in
+        cons_uniq v types
+      | fun x => ?e =>
+        collectTypes_expr e types
+      | _ =>
+        let rec bt_args args types :=
+          match args with
+            | tt => types
+            | (?a, ?b) =>
+              let types := collectTypes_expr a types in
+              bt_args b types
+          end
+        in
+        let cc _ Ts args := 
+          let T := 
+            match e with 
+              | fun x : VarType _ => _ => 
+                match type of e with
+                  | _ -> ?T => T
+                end
+              | _ => type of e
+            end
+          in
+          let Ts :=
+            let v := constr:(T : Type) in
+            cons_uniq v Ts 
+          in
+          let types := append_uniq Ts types in
+          bt_args args types
+        in
+        refl_app cc e
+    end.
+
+  Ltac map_non_dep ty args f acc :=
+    match args with
+      | tt => acc
+      | (?A1, ?A2) =>
+        match ty with
+          | ?T1 -> ?T2 =>
+            let acc := f T1 A1 acc in
+            map_non_dep T2 A2 f acc
+          | forall x : ?T1, @?T2 x =>
+            match A1 with
+              | fun _ => ?A => 
+                let t := eval simpl in (T2 A) in
+                map_non_dep t A2 f acc
+            end
+          | _ => acc
+        end
+    end.
+
+  Ltac collectTypes_sexpr s types k :=
+    match s with
+      | fun x : VarType ?T => @ST.star _ _ _ (@?L x) (@?R x) =>
+        collectTypes_sexpr L types ltac:(fun types =>
+          collectTypes_sexpr R types k)
+      | fun x : ?T => @ST.ex _ _ _ ?T' (fun y : ?T' => @?B x y) =>
+        let v := constr:(fun x : VarType (T * T') => 
+          B (@openUp _ T (@fst _ _) x) (@openUp _ T' (@snd _ _) x)) in
+        let v := eval simpl in v in
+        collectTypes_sexpr v types k
+      | @ST.emp _ _ _ => k types
+      | @ST.inj _ _ _ (PropX.Inj _ _ _ ?P) =>
+        k ltac:(collectTypes_expr P types)
+      | @ST.inj _ _ _ ?PX => k types
+      | @ST.star _ _ _ ?L ?R =>
+        collectTypes_sexpr L types
+          ltac:(fun Ltypes => collectTypes_sexpr R Ltypes k)
+      | @ST.ex _ _ _ ?T (fun x : ?T => @?B x) =>
+        let v := constr:(fun x : VarType T => B (@openUp _ T (fun x => x) x)) in
+        let v := eval simpl in v in 
+        collectTypes_sexpr v types k
+      | ?X =>
+        let rec bt_args args types :=
+          match args with
+            | tt => k types
+            | (?a,?b) => 
+              let k := collectTypes_expr a types in
+              bt_args b k
+          end
+        in
+        let cc _ Ts args := 
+          let types := append_uniq Ts types in
+          bt_args args types
+        in
+        refl_app cc X
+    end.
+
+  Ltac indexOf_nat proj x xs :=
+    let rec search xs :=
+      match xs with
+        | ?X :: ?XS =>
+          let X' := eval simpl in (proj X) in
+          match X' with
+            | x => constr:(0)
+            | _ => 
+              let r := search XS in
+              constr:(S r)
+          end
+      end
+    in search xs.
+
+  Ltac typesIndex x types :=
+    indexOf_nat Impl x types.
+
+  Ltac reflectType types t :=
+    match t with
+      | Prop => constr:(tvProp)
+      | _ =>
+        let i := typesIndex t types in
+        let r := constr:(tvType i) in
+        r
+    end.  
+        
+  Ltac reflectTypes_toList types ts :=
+    match ts with 
+      | nil => constr:(@nil tvar)
+      | ?T :: ?TS =>
+        let i := typesIndex T types in
+        let rest := reflectTypes_toList types TS in
+        constr:(@cons tvar (tvType i) rest)
+    end.
+
+  Ltac collectAllTypes isConst ts goals :=
+    match goals with
+      | nil => ts
+      | ?a :: ?b =>
+        (** TODO : I may need to reflect the pcType and stateType **)
+        let ts := collectTypes_sexpr a ts ltac:(fun ts => ts) in
+        collectAllTypes isConst ts b
+    end.
+
+  Ltac getVar idx vars :=
+    match vars with
+      | nil => idtac "empty variable list!" idx
+      | ?a :: ?b =>
+        match idx with
+          | fun x => @openUp _ _ (@fst _ _) _ =>
+            constr:(0)
+          | fun x => @openUp _ _ (@snd _ _) (@?X x) =>
+            let r := getVar X vars in
+            constr:(S r)
+          | _ => idtac "couldn't find variable!" idx vars
+        end
+    end.
+
+  Ltac reflect_function types f :=
+    let T := type of f in
+    let rec refl dom T :=
+      match T with
+        (* no dependent types *)
+        | ?A -> ?B =>
+          let A := reflectType types A in
+          let dom := constr:(A :: dom) in
+          refl dom B 
+        | ?R =>
+          let R := reflectType types R in
+          let dom := eval simpl rev in (rev dom) in
+          constr:(@Build_signature types dom R f)
+      end
+   in refl (@nil tvar) T.
+
+
+  Ltac getFunction types f funcs k :=
+    let rec lookup funcs acc :=
+      match funcs with
+        | nil =>
+          let F := reflect_function types f in
+          let funcs := eval simpl app in (funcs ++ (F :: nil)) in
+          k funcs acc
+        | ?F :: ?FS =>
+          let F' := eval simpl Denotation in (Denotation F) in
+          match F' with
+            | f => k funcs acc
+            | _ => 
+              let acc := constr:(S acc) in
+              lookup FS acc
+          end
+      end
+    in lookup funcs 0.
+
+  (** reflect an expression gathering the functions at the same time.
+   ** - k funcs expr
+   **)
+  Ltac reflect_expr isConst e types funcs uvars vars k :=
+    let rec reflect funcs e k :=
+      match e with
+        | fun _ => ?X =>
+          is_evar X ; 
+          (** this is a unification variable **)
+          let r := constr:(@Expr.UVar) in (** TODO **)
+          k funcs r 
+        | fun x => (@openUp _ _ _ _) =>
+          (** this is a variable **)
+          let v := getVar e vars in
+          let r := constr:(@Expr.Var types funcs uvars vars v) in
+          k funcs r
+        | fun x => ?e =>
+          reflect funcs e k
+        | _ =>
+          let rec bt_args funcs args k :=
+            match args with
+              | tt => 
+                let v := constr:(@nil (@expr types)) in
+                k funcs v
+              | (?a, ?b) =>
+                reflect funcs a ltac:(fun funcs a =>
+                  bt_args funcs b ltac:(fun funcs b =>
+                    let r := constr:(@cons (@expr types) a b) in
+                    k funcs r))
+            end
+          in
+          let cc f Ts args :=
+            getFunction types f funcs ltac:(fun funcs F =>
+              bt_args funcs args ltac:(fun funcs args =>
+                let r := constr:(@Expr.Func types F args) in 
+                k funcs r))
+          in
+          match e with
+            | _ => 
+              match isConst e with
+                | true => 
+                  let ty := type of e in
+                  let ty := reflectType types ty in
+                  let r := eval simpl in (@Expr.Const types ty e) in
+                  k funcs r
+                | false => 
+                  refl_app cc e
+              end
+            | _ => refl_app cc e
+          end
+      end
+    in reflect funcs e k.
+
+  Ltac reflect_sfunction pcT stT types f :=
+    let T := type of f in
+    let rec refl dom T :=
+      match T with
+        (* no dependent types *)
+        | ?A -> ?B =>
+          let A := reflectType types A in
+          let dom := constr:(A :: dom) in
+          refl dom B 
+        | _ =>
+          let dom := eval simpl rev in (rev dom) in
+          constr:(@Build_ssignature types pcT stT dom f)
+      end
+   in refl (@nil tvar) T.
+
+  Ltac getSFunction pcT stT types f sfuncs k :=
+    let rec lookup sfuncs' acc :=
+      match sfuncs' with
+        | nil =>
+          let F := reflect_sfunction pcT stT types f in
+          let sfuncs := eval simpl app in (sfuncs ++ (F :: nil)) in
+          k sfuncs acc
+        | ?F :: ?FS =>
+          let F' := eval simpl SDenotation in (SDenotation F) in
+          match F' with
+            | f => 
+              k sfuncs acc 
+            | _ => 
+              let acc := constr:(S acc) in
+              lookup FS acc
+          end
+      end
+    in lookup sfuncs 0.
+
+
+  (** reflect sexprs. simultaneously gather the funcs and sfuncs
+   ** k funcs sfuncs sexpr
+   **)
+  Ltac reflect_sexpr isConst s types funcs pcType stateType sfuncs uvars vars k :=
+    let implicits ctor :=
+      constr:(ctor types pcType stateType)
+    in
+    let rec reflect s funcs sfuncs uvars vars k :=
+      match s with
+        | fun _ => ?s =>
+          reflect s funcs sfuncs uvars vars k
+        | fun x : VarType ?T => @ST.star _ _ _ (@?L x) (@?R x) =>
+          reflect L funcs sfuncs uvars vars ltac:(fun funcs sfuncs L =>
+            reflect R funcs sfuncs uvars vars ltac:(fun funcs sfuncs R => 
+              let r := constr:(@Star) in
+              let r := implicits r in
+              let r := constr:(r L R) in
+              k funcs sfuncs r))
+        | fun x : ?T => @ST.ex _ _ _ ?T' (fun y : ?T' => @?B y x) =>
+          let v := constr:(fun x : VarType (T' * T) => 
+            B (@openUp _ T (@fst _ _) x) (@openUp _ T' (@snd _ _) x)) in
+          let v := eval simpl in v in
+          let vars' := 
+            let nv := reflectType types T' in
+            constr:(nv :: vars)
+          in
+          reflect v funcs sfuncs uvars vars' ltac:(fun funcs sfuncs B =>
+            let r := constr:(@Exists) in
+            let r := implicits r in
+            let r := constr:(@r _ B) in
+            k funcs sfuncs r)
+        | @ST.emp _ _ _ => 
+          let r := constr:(@Emp) in
+          let r := implicits r in
+          k funcs sfuncs r
+
+        | @ST.inj _ _ _ (PropX.Inj _ _ _ ?P) =>
+          reflect_expr isConst P types funcs uvars vars ltac:(fun funcs P =>
+            let r := constr:(@Inj) in
+            let r := implicits r in
+            let r := constr:(r P) in
+            k funcs sfuncs r)
+        | @ST.inj _ _ _ ?PX =>
+          let r := constr:(@Const) in
+          let r := implicits r in
+          let r := constr:(r PX) in
+          k funcs sfuncs r
+        | @ST.star _ _ _ ?L ?R =>
+          reflect L funcs sfuncs uvars vars ltac:(fun funcs sfuncs L => 
+            reflect R funcs sfuncs uvars vars ltac:(fun funcs sfuncs R => 
+              let r := constr:(@Star) in
+              let r := implicits r in
+              let r := constr:(r L R) in
+              k funcs sfuncs r))
+        | @ST.ex _ _ _ ?T (fun x : ?T => @?B x) =>
+          let v := constr:(fun x : VarType (T * unit) => B (@openUp _ T (@fst _ _) x)) in
+          let v := eval simpl in v in
+          let vars' := 
+            let nv := reflectType types T in
+            constr:(nv :: vars)
+          in
+          reflect v funcs sfuncs uvars vars' ltac:(fun funcs sfuncs B =>
+            let r := constr:(@Exists) in
+            let r := implicits r in
+            let r := constr:(@r _ B) in
+            k funcs sfuncs r)
+        | ?X =>
+          let rec bt_args args funcs k :=
+            match args with
+              | tt => 
+                let v := constr:(@nil (@expr types)) in
+                k funcs v
+              | (?a,?b) =>
+                reflect_expr isConst a types funcs uvars vars ltac:(fun funcs a =>
+                  bt_args b funcs ltac:(fun funcs b => 
+                  let v := constr:(@cons (@expr types) a b) in
+                  k funcs v))
+            end
+          in
+          let cc f Ts As :=
+            getSFunction pcType stateType types f sfuncs ltac:(fun sfuncs F =>
+            bt_args As funcs ltac:(fun funcs args =>
+            let r := constr:(@Func) in
+            let r := implicits r in
+            let r := constr:(@r F args) in
+            k funcs sfuncs r))
+          in
+          refl_app cc X
+      end
+    in
+    reflect s funcs sfuncs uvars vars k.
+
+  Ltac reflect_all pcT stT isConst Ts goals := 
+    let rt := 
+      collectAllTypes isConst ((pcT : Type) :: (stT : Type) :: @nil Type) goals
+    in
+    let Ts := extend_all_types rt Ts in
+    let Ts := eval simpl in Ts in
+    let pcTyp := typesIndex pcT Ts in
+    let stTyp := typesIndex stT Ts in
+    let pcTyp := constr:(tvType pcTyp) in
+    let stTyp := constr:(tvType stTyp) in
+    let fs := constr:(@nil (@signature Ts)) in
+    let sfs := constr:(@nil (@ssignature Ts pcTyp stTyp)) in
+    let rec reflect_all ls funcs sfuncs k :=
+      match ls with
+        | nil => 
+          let r := constr:(@nil (@sexpr Ts pcTyp stTyp)) in
+          k funcs sfuncs r
+        | ?e :: ?es =>
+          let vs := constr:(@nil tvar) in
+          let us := constr:(@nil tvar) in
+          reflect_sexpr isConst e Ts funcs pcTyp stTyp sfuncs us vs ltac:(fun funcs sfuncs e =>
+            reflect_all es funcs sfuncs ltac:(fun funcs sfuncs es =>
+              let es := constr:(e :: es) in
+              k funcs sfuncs es)) 
+      end
+    in
+    reflect_all goals fs sfs ltac:(fun funcs sfuncs es =>
+      constr:((Ts, pcTyp, stTyp, funcs, sfuncs, es))).
+    
+(*
+    match collectAllFunctions build_ssig isConst goals Ts fs sfs with
+      | (?funcs, ?sfuncs) =>
+        let goals := reflectAll isConst goals Ts pcTyp stTyp funcs sfuncs in
+        goals
+    end.
+*)
+
+  Section Tests.
+    Variable f : forall a b, nat -> ST.hprop a b nil.
+    Variable h : forall a b, nat -> ST.hprop a b nil.
+    Variable i : forall a b, nat -> ST.hprop a b nil.
+    Variable g : bool -> nat -> nat -> nat.
+
+    Variable a : Type.
+    Variable b : Type.
+    
+    Definition hpropB : list Type -> Type := ST.hprop a b.
+
+    Variable p : forall {sos}, nat -> nat -> hpropB sos.
+
+    Ltac isConst e :=
+      match e with
+        | true => true
+        | false => true
+        | O => true
+        | S ?e => isConst e
+        | _ => false
+      end.
+
+    Definition nat_type : type :=
+      {| Impl := nat 
+       ; Eq := fun x y => match equiv_dec x y with
+                            | left pf => Some pf
+                            | _ => None 
+                          end
+       |}.
+
+    Lemma change_ST_himp_himp : forall (types : list type)
+      (funcs : functions types) (pc st : tvar)
+      (sfuncs : list (ssignature types pc st))
+      
+      (cs : codeSpec (tvarD types pc) (tvarD types st))
+      (L R : sexpr types pc st),
+      himp funcs sfuncs nil nil nil cs L R ->
+      match 
+        @sexprD types funcs pc st sfuncs L nil nil , 
+        @sexprD types funcs pc st sfuncs R nil nil
+        with
+        | Some l , Some r => 
+          ST.himp cs l r
+        | _ , _ => False
+      end.
+    Proof.
+      unfold himp. intros. 
+      destruct (sexprD funcs sfuncs L nil nil);
+        destruct (sexprD funcs sfuncs R nil nil); auto.
+    Qed.
+
+    Implicit Arguments Expr.Const [ types t ].
+
+    Opaque himp.
+
+    Goal forall c x, @ST.himp a b c (p nil 1 x) (p _ 1 x).
+      intros.
+      match goal with
+        | [ |- @ST.himp ?p ?s ?cs ?L ?R ] =>
+          let r := reflect_all p s isConst (nat_type :: nil) (L :: R :: nil) in
+          match r with
+            | (?types, ?pcTyp, ?stTyp, ?fs, ?sfs, ?L :: ?R :: nil) =>
+              apply (@change_ST_himp_himp types fs pcTyp stTyp sfs cs L R)
+          end
+      end.
+    Abort.
+
+(*
+      Lemma ApplyCancelSep : forall cs l r res,
+        res = CancelSep cs nil l r ->
+(*          | Prove vars u2 l' r' SUBST _ => *)
+            forallEach
+            (fun VS : hlist (@tvarD types) vars =>
+              exists_subst VS SUBST
+              (fun k : hlist (@tvarD types) u2 => himp HNil k VS cs l' r'))
+(* -> *)
+        himp nil nil nil cs l r.
+      Proof.
+        clear. intros. destruct (CancelSep cs nil l r). auto.
+      Qed.
+*)      
+
+
+    Fixpoint all a b (f : nat -> ST.hprop a b nil) (n : nat) : ST.hprop a b nil :=
+      match n with
+        | 0 => f 0
+        | S n => ST.star (f (S n)) (all f n)
+      end.
+
+    Fixpoint allb a b (f : nat -> ST.hprop a b nil) (n m : nat) : ST.hprop a b nil :=
+      match n with
+        | 0 => f m
+        | S n => ST.star (f (m - S n)) (allb f n m)
+      end.
+
+
+    Goal forall c, @ST.himp a b c 
+      (ST.star (allb (@h a b) 15 15) (allb (@f a b) 15 15))
+      (ST.star (all (@f a b) 15) (all (@h a b) 15)).
+      simpl all. simpl allb.
+      intros. 
+      match goal with
+        | [ |- @ST.himp ?p ?s ?cs ?L ?R ] =>
+          let r := reflect_all p s isConst (nat_type :: nil) (L :: R :: nil) in
+          match r with
+            | (?types, ?pcTyp, ?stTyp, ?fs, ?sfs, ?L :: ?R :: nil) =>
+              apply (@change_ST_himp_himp types fs pcTyp stTyp sfs cs L R)
+          end
+      end.
+    Abort.
+End Tests.
+
+
 End SepExpr.
